theories/Monad/EitherMonad.v
@@ -1,0 +1,62 @@
+Require Import Monad.
+
+Section except.
+  Variable T : Type.
+  
+  Global Instance Monad_either : Monad (sum T) :=
+  { ret  := fun _ v => inr v
+  ; bind := fun _ c1 _ c2 => match c1 with 
+                               | inl v => inl v
+                               | inr v => c2 v
+                             end 
+  }.
+
+  Global Instance Exception_either : MonadExc T (sum T) :=
+  { raise := fun v _ => inl v
+  ; catch := fun _ c h => match c with
+                            | inl v => h v
+                            | x => x
+                          end
+  }.
+
+  Variable m : Type -> Type.
+
+  Definition eitherT : Type -> Type := 
+    fun x => m (sum T x).
+
+  Variable M : Monad m.
+
+  Global Instance Monad_eitherT : Monad eitherT :=
+  { ret := fun _ x => @ret m M _ (inr x)
+  ; bind := fun _ c1 _ c2 =>
+    @bind _ M _ c1 _ (fun c1 =>
+      match c1 with
+        | inl x => @ret _ M _ (inl x)
+        | inr v => c2 v
+      end)
+  }.
+
+  Global Instance Exception_eitherT : MonadExc T eitherT :=
+  { raise := fun v _ => @ret _ M _ (inl v)
+  ; catch := fun _ c h =>
+    bind (Monad := M) c (fun e_v =>
+      match e_v with
+        | inl x => h x
+        | inr x => ret (inr x)
+      end)
+  }.
+
+  Global Instance MonadT_eitherT : MonadT eitherT m :=
+  { lift := fun _ c => bind c (fun x => ret (ret x)) }.
+
+  Global Instance State_eitherT {T} (SM : State T m) : State T eitherT :=
+  { get := lift get 
+  ; put := fun v => lift (put v)
+  }.
+
+  Global Instance Reader_eitherT {T} (SM : Reader T m) : Reader T eitherT :=
+  { ask := lift ask
+  ; local := fun v T cmd => local (Reader := SM) v cmd 
+  }.
+
+End except.
